SetTheory/lean/SetTheory/PAHF.lean
@@ -22,3 +22,4 @@ import SetTheory.PAHF.PASyntax
 import SetTheory.PAHF.RiemannHypothesis
 import SetTheory.PAHF.Interpretation
 import SetTheory.PAHF.RoundTrip
+import SetTheory.PAHF.HFRoundTrip
